src/examples/fractional.v
@@ -23,7 +23,6 @@ From lang Require Import lang.
 From iris Require Import options.
 
 Require Import guarding.guard.
-Require Import guarding.guard_later.
 Require Import guarding.storage_protocol.protocol.
 Require Import guarding.storage_protocol.inved.
 From iris.algebra Require Import auth.
